- Added lambda lifting - Changed the namespace of files in Libraries (to Libraries instead of “”) because of name clashes with files in compcert.lib. There are redundancies between the two directories that we should fix at some point. Remember to recompile Libraries. - Changed (all?) L6 imports to qualified ones - Commented out from _CoqProject files that do not currently compile

theories/L6_PCPS/functions.v
@@ -1,6 +1,7 @@
-Require Import Coq.Numbers.BinNums Coq.NArith.BinNat Coq.PArith.BinPos Coqlib Coq.Sets.Ensembles
+Require Import L6.Ensembles_util.
+Require Import Libraries.Coqlib.
+Require Import Coq.Numbers.BinNums Coq.NArith.BinNat Coq.PArith.BinPos Coq.Sets.Ensembles
         Coq.Relations.Relations Coq.Classes.Morphisms.
-Require Import Ensembles_util.
 
 (** ** Usefull definitions and lemmas about functions. *)
 
@@ -26,7 +27,7 @@ Definition f_eq  {A B} (f1 f2 : A -> B) : Prop :=  forall x, f1 x = f2 x.
 (** Extend a function. Only works for positives to avoid parameterizing the definition with
   * the decidable equality proof. TODO: fix this *)
 Definition extend (f: positive -> positive) (x x' : positive) : (positive -> positive) :=
-  fun z => if Coqlib.peq z x then x' else f z.
+  fun z => if peq z x then x' else f z.
 
 Notation " f '{' x '~>' y '}' " := (extend f x y) (at level 10, no associativity)
                                    : fun_scope.
@@ -153,27 +154,27 @@ Qed.
 Instance extend_Proper : Proper (f_eq ==> Logic.eq ==> Logic.eq ==> f_eq) extend.
 Proof. 
   intros f1 f2 Hfeq x1 x2 Heq1 x3 x4 Hfeq2; subst.
-  intros x. unfold extend. destruct (Coqlib.peq x x2); eauto.
+  intros x. unfold extend. destruct (peq x x2); eauto.
 Qed.
 
 Lemma extend_gss f x x' :
   f {x ~> x'} x = x'.
 Proof. 
-  unfold extend. rewrite Coqlib.peq_true. reflexivity.
+  unfold extend. rewrite peq_true. reflexivity.
 Qed.
 
 Lemma extend_gso f x x' y :
   y <> x ->
   f {x ~> x'} y = f y.
 Proof. 
-  intros Heq. unfold extend. rewrite Coqlib.peq_false; eauto.
+  intros Heq. unfold extend. rewrite peq_false; eauto.
 Qed.
 
 Lemma extend_same f x y :
   f x = x ->
   f {y ~> y} x = x. 
 Proof.
-  unfold extend. destruct (Coqlib.peq x y); eauto.
+  unfold extend. destruct (peq x y); eauto.
 Qed.
 
 Lemma f_eq_extend (f f' : positive -> positive) x y :
@@ -182,7 +183,7 @@ Lemma f_eq_extend (f f' : positive -> positive) x y :
 Proof. 
   intros Heq. 
   unfold extend. intros z. 
-  destruct (Coqlib.peq z x); eauto.
+  destruct (peq z x); eauto.
 Qed.
 
 Lemma f_eq_extend_same (f : positive -> positive) x y :
@@ -190,7 +191,7 @@ Lemma f_eq_extend_same (f : positive -> positive) x y :
   f_eq (f{x ~> y}) f.
 Proof. 
   intros Heq x'.
-    unfold extend. destruct (Coqlib.peq x' x); eauto.
+    unfold extend. destruct (peq x' x); eauto.
     congruence. 
 Qed.    
 
@@ -200,7 +201,7 @@ Lemma f_eq_subdomain_extend S (f f' : positive -> positive) x y :
 Proof. 
   intros Heq. 
   unfold extend. intros z Hin. 
-  destruct (Coqlib.peq z x). now eauto.
+  destruct (peq z x). now eauto.
   apply Heq. inv Hin; [| now eauto ]. inv H; congruence. 
 Qed.
 
@@ -243,13 +244,13 @@ Lemma image_extend_In_S f x x' S :
 Proof.
   intros HinS. split. 
   - intros y [y' [Hin Heq]]; subst. 
-    destruct (Coqlib.peq x y').
+    destruct (peq x y').
     + subst. rewrite extend_gss. eauto.
     + rewrite extend_gso; eauto. left.
       eexists; split; eauto. constructor; eauto.
       intros Hc; inv Hc; congruence.
   - intros y Hin.
-    destruct (Coqlib.peq x' y); subst.
+    destruct (peq x' y); subst.
     + eexists; split; eauto. rewrite extend_gss; eauto.
     + inv Hin. 
       * destruct H as [y' [Hin Heq]]; subst. inv Hin.
@@ -272,7 +273,7 @@ Lemma image_extend_Included f x x' S :
   Included _ (image (f {x ~> x'}) S) (Union _ (image f S) (Singleton _ x')).
 Proof.  
   intros y [y' [Hin Heq]]. unfold extend in Heq.
-  destruct (Coqlib.peq y' x); subst; [ now eauto |] .
+  destruct (peq y' x); subst; [ now eauto |] .
   left. eexists; eauto.
 Qed.
 
@@ -362,15 +363,15 @@ Lemma injective_subdomain_extend f x x' S :
 Proof.
   intros Hinj Hnin.
   intros y y' Hin1 Hin2.
-  destruct (Coqlib.peq x y); subst.
+  destruct (peq x y); subst.
   - rewrite extend_gss. intros Heq.
-    destruct (Coqlib.peq y y'); [ now eauto | ].
+    destruct (peq y y'); [ now eauto | ].
     rewrite extend_gso in Heq; [| now eauto ]. 
     exfalso. eapply Hnin. eexists; split; [| now eauto ].
     inv Hin2. inv H. congruence.
     constructor; eauto. intros Hc; inv Hc; congruence.
   - rewrite extend_gso; [| now eauto ].
-    destruct (Coqlib.peq x y'); subst.
+    destruct (peq x y'); subst.
     + rewrite extend_gss. intros Heq. subst.
       exfalso. apply Hnin. eexists.
       split; [| reflexivity ].
@@ -389,14 +390,14 @@ Lemma injective_subdomain_extend' f x x' S :
 Proof.
   intros Hinj Hnin.
   intros y y' Hin1 Hin2.
-  destruct (Coqlib.peq x y); subst.
+  destruct (peq x y); subst.
   - rewrite extend_gss. intros Heq.
-    destruct (Coqlib.peq y y'); [ now eauto | ].
+    destruct (peq y y'); [ now eauto | ].
     rewrite extend_gso in Heq; [| now eauto ]. 
     exfalso. eapply Hnin. eexists; split; [| now eauto ].
     constructor; eauto. intros Hc; eapply n. now inv Hc.
   - rewrite extend_gso; [| now eauto ].
-    destruct (Coqlib.peq x y'); subst.
+    destruct (peq x y'); subst.
     + rewrite extend_gss. intros Heq. subst.
       exfalso. apply Hnin. eexists.
       split; [| reflexivity ].
@@ -412,11 +413,11 @@ Lemma injective_extend (f : positive -> positive) x y :
 Proof.
   intros Hinj Hin x1 x2 __ _ Heq.
   unfold extend in *.
-  edestruct (Coqlib.peq x1 x).
+  edestruct (peq x1 x).
   - rewrite <- e in Heq.
-    edestruct (Coqlib.peq x2 x1); [ now eauto |].
+    edestruct (peq x2 x1); [ now eauto |].
     exfalso. eapply Hin. eexists; eauto.
-  - edestruct (Coqlib.peq x2 x).
+  - edestruct (peq x2 x).
     + exfalso. eapply Hin. eexists; eauto.
     + eapply Hinj; try now constructor; eauto.
       assumption.
