theories/L6_PCPS/L6_compose.v
@@ -1,7 +1,7 @@
-Require Import cps ctx cps_util List_util eval identifiers functions hoare Ensembles_util
-        closure_conversion closure_conversion_correct closure_conversion_corresp
-        hoisting logical_relations.
-(* Require Import Coq.ZArith.Znumtheory Coq.Relations.Relations Coq.Arith.Wf_nat. *)
+Require Import L6.cps L6.ctx L6.cps_util L6.List_util L6.eval L6.identifiers
+        L6.functions L6.hoare L6.Ensembles_util L6.closure_conversion
+        L6.closure_conversion_correct L6.closure_conversion_corresp L6.hoisting
+        L6.logical_relations.
 Require Import Coq.Lists.List Coq.MSets.MSets Coq.MSets.MSetRBT Coq.Numbers.BinNums
         Coq.NArith.BinNat Coq.PArith.BinPos Coq.Sets.Ensembles Omega.
 Require Import ExtLib.Structures.Monads ExtLib.Data.Monads.StateMonad.
