theories/L6_PCPS/cps_util.v
@@ -1,8 +1,8 @@
 Require Import Coq.Arith.Arith Coq.NArith.BinNat Coq.Strings.String Coq.Lists.List
         Coq.omega.Omega Coq.Sets.Ensembles Coq.Relations.Relation_Operators.
 
-Require Import CpdtTactics.
-Require Import cps ctx eval Ensembles_util List_util.
+Require Import Libraries.CpdtTactics.
+Require Import L6.cps L6.ctx L6.eval L6.Ensembles_util L6.List_util.
 
 Import ListNotations.
 
