theories/L6_PCPS/.dir-locals.el
@@ -1,1 +1,5 @@
-((coq-mode . ((coq-prog-args . ("-emacs-U" "-R" "../../libraries" "")))))
+((coq-mode . ((coq-load-path . (
+                                (rec "../../libraries" "Libraries")
+                                (rec "../L6_PCPS" "L6")
+                                (rec "../common" "Common")
+                                )))))
